Progress on removing cheats from loopProps

pancake/crep_to_loopScript.sml
@@ -1,11 +1,172 @@
 (*
   Compilation from crepLang to panLang.
 *)
-open preamble crepLangTheory loopLangTheory
+open preamble crepLangTheory
+     loopLangTheory sptreeTheory
 
 val _ = new_theory "crep_to_loop"
 
-val _ = set_grammar_ancestry ["crepLang","loopLang", "backend_common"];
+val _ = set_grammar_ancestry
+        ["crepLang", "loopLang",
+         "backend_common", "sptree"];
 
+Datatype:
+  context =
+  <| vars    : crepLang$varname |-> num;
+     funcs   : crepLang$funname |-> num # num list;  (* loc, args *)
+     ceids    : ('a word) list;
+     vmax : num|>
+End
+
+Definition find_var_def:
+  find_var ct v =
+   case FLOOKUP ct.vars v of
+    | SOME n => n
+    | NONE => 0
+End
+
+Definition find_lab_def:
+  find_lab ct f =
+   case FLOOKUP ct.funcs f of
+    | SOME (n, _) => n
+    | NONE => 0
+End
+
+Definition prog_if_def:
+  prog_if cmp p q e e' n m l =
+   p ++ q ++ [
+    Assign n e; Assign m e';
+    If cmp n (Reg m)
+    (Assign n (Const 1w)) (Assign n (Const 0w)) (list_insert [n; m] l)]
+End
+
+Definition compile_exp_def:
+  (compile_exp ctxt tmp l ((Const c):'a crepLang$exp) = ([], Const c, tmp, l)) /\
+  (compile_exp ctxt tmp l (Var v) = ([], Var (find_var ctxt v), tmp, l)) /\
+  (compile_exp ctxt tmp l (Label f) = ([LocValue tmp (find_lab ctxt f)],
+                                       Var tmp, tmp + 1, insert tmp () l)) /\
+  (compile_exp ctxt tmp l (Load ad) =
+   let (p, le, tmp, l) = compile_exp ctxt tmp l ad in (p, Load le, tmp, l)) /\
+  (compile_exp ctxt tmp l (LoadByte ad) =
+   let (p, le, tmp, l) = compile_exp ctxt tmp l ad in
+    (p ++ [Assign tmp le; LoadByte tmp tmp], Var tmp, tmp + 1, insert tmp () l)) /\
+  (compile_exp ctxt tmp l (LoadGlob gadr) = ([], Lookup gadr, tmp, l)) /\
+  (compile_exp ctxt tmp l (Op bop es) =
+   let (p, les, tmp, l) = compile_exps ctxt tmp l es in
+   (p, Op bop les, tmp, l)) /\
+  (compile_exp ctxt tmp l (Cmp cmp e e') =
+   let (p, le, tmp, l) = compile_exp ctxt tmp l e in
+   let (p', le', tmp', l) = compile_exp ctxt tmp l e' in
+     (prog_if cmp p p' le le' (tmp' + 1) (tmp' + 2) l, Var (tmp' + 1), tmp' + 3,
+      list_insert [tmp' + 1; tmp' + 2] l)) /\
+  (compile_exp ctxt tmp l (Shift sh e n) =
+   let (p, le, tmp, l) = compile_exp ctxt tmp l e in (p, Shift sh le n, tmp, l)) /\
+
+  (compile_exps ctxt tmp l cps = (* to generate ind thm *)
+   case cps of
+   | [] => ([], [], tmp, l)
+   | e::es =>
+     let (p, le, tmp, l) = compile_exp ctxt tmp l e in
+      let (p1, les, tmp, l) = compile_exps ctxt tmp l es in
+      (p ++ p1, le::les, tmp, l))
+Termination
+  cheat
+End
+
+Definition gen_temps_def:
+  gen_temps n l = GENLIST (\x. n + x) l
+End
+
+Definition rt_exp_var_def:
+  rt_exp_var fm NONE (n:num) = n /\
+  rt_exp_var fm (SOME v) n =
+    case FLOOKUP fm v of
+     | NONE => 0 (* impossible *)
+     | SOME m => m
+End
+
+
+Definition compile_prog_def:
+  (compile_prog _ _ (Skip:'a crepLang$prog) = (Skip:'a loopLang$prog)) /\
+  (compile_prog _ _ Break = Break) /\
+  (compile_prog _ _ Continue = Continue) /\
+  (compile_prog _ _ Tick = Tick) /\
+  (compile_prog ctxt l (Return e) =
+    let (p, le, ntmp, nl) = compile_exp ctxt (ctxt.vmax + 1) l e in
+      nested_seq (p ++ [Assign ntmp le; Return ntmp])) /\
+  (compile_prog ctxt l (Raise eid) =
+    Seq (Assign (ctxt.vmax + 1) (Const eid)) (Raise (ctxt.vmax + 1))) /\
+  (compile_prog ctxt l (Store dst src) =
+    let (p, le, tmp, l) = compile_exp ctxt (ctxt.vmax + 1) l dst in
+      let (p', le', tmp, l) = compile_exp ctxt tmp l src in
+        nested_seq (p ++ p' ++ [Assign tmp le'; Store le tmp])) /\
+  (compile_prog ctxt l (StoreByte dst src) =
+    let (p, le, tmp, l) = compile_exp ctxt (ctxt.vmax + 1) l dst in
+      let (p', le', tmp, l) = compile_exp ctxt tmp l src in
+        nested_seq (p ++ p' ++
+                     [Assign tmp le; Assign (tmp + 1) le';
+                      StoreByte tmp (tmp + 1)])) /\
+  (compile_prog ctxt l (StoreGlob adr e) =
+    let (p, le, tmp, l) = compile_exp ctxt (ctxt.vmax + 1) l e in
+        nested_seq (p ++ [SetGlobal adr le])) /\
+  (compile_prog ctxt l (Seq p q) =
+    Seq (compile_prog ctxt l p) (compile_prog ctxt l q)) /\
+  (compile_prog ctxt l (Assign v e) =
+    case FLOOKUP ctxt.vars v of
+     | SOME n =>
+       let (p,le,tmp, l) = compile_exp ctxt (ctxt.vmax + 1) l e in
+        nested_seq (p ++ [Assign n le])
+     | NONE => Skip) /\
+  (compile_prog ctxt l (Dec v e prog) =
+    let (p,le,tmp,nl) = compile_exp ctxt (ctxt.vmax + 1) l e;
+         nctxt = ctxt with <|vars := ctxt.vars |+ (v,tmp);
+                             vmax := tmp|>;
+         fl = insert tmp () l;
+         lp = compile_prog nctxt fl prog in
+     Seq (nested_seq p) (Seq (Assign tmp le) lp)) /\
+  (compile_prog ctxt l (If e p q) =
+    let (np, le, tmp, nl) = compile_exp ctxt (ctxt.vmax + 1) l e;
+        lp = compile_prog ctxt l p;
+        lq = compile_prog ctxt l q in
+    nested_seq (np ++ [Assign tmp le;
+                       If NotEqual tmp (Imm 0w) lp lq l])) /\
+
+  (compile_prog ctxt l (While e p) =
+    let (np, le, tmp, nl) = compile_exp ctxt (ctxt.vmax + 1) l e;
+        lp = compile_prog ctxt l p in
+     Loop l (nested_seq (np ++ [
+                Assign tmp le;
+                If NotEqual tmp (Imm 0w)
+                   (Seq lp Continue) Break l]))
+          l) /\
+  (compile_prog ctxt l (Call Tail e es) =
+   let (p, les, tmp, nl) = compile_exps ctxt (ctxt.vmax + 1) l (es ++ [e]);
+       nargs = gen_temps tmp (LENGTH les) in
+   nested_seq (p ++ MAP2 Assign nargs les ++
+               [Call NONE NONE nargs NONE])) /\
+
+
+  (compile_prog ctxt l (Call (Ret rt rp hdl) e es) =
+   let (p, les, tmp, nl) = compile_exps ctxt (ctxt.vmax + 1) l (es ++ [e]);
+       nargs = gen_temps tmp (LENGTH les);
+       rn  = rt_exp_var ctxt.vars rt (ctxt.vmax + 1);
+       en  = ctxt.vmax + 1;
+       pr  = compile_prog ctxt l rp;
+       pe  = case hdl of
+              | NONE => Raise en
+              | SOME (Handle eid ep) =>
+                let cpe = compile_prog ctxt l ep in
+                if ~MEM eid ctxt.ceids then (Raise en)
+                else (If NotEqual en (Imm eid) (Raise en) (Seq Tick cpe) l) in
+      nested_seq (p ++ MAP2 Assign nargs les ++
+               [Call (SOME (rn, l)) NONE nargs
+                     (SOME (en, pe, pr, l))])) /\
+  (compile_prog ctxt l (ExtCall f ptr1 len1 ptr2 len2) =
+    case (FLOOKUP ctxt.vars ptr1, FLOOKUP ctxt.vars len1,
+          FLOOKUP ctxt.vars ptr2, FLOOKUP ctxt.vars len2) of
+     | (SOME pc, SOME lc, SOME pc', SOME lc') =>
+         FFI (explode f) pc lc pc' lc' l
+     | _ => Skip)
+End
 
 val _ = export_theory();
