pancake/semantics/loopPropsScript.sml
@@ -50,6 +50,45 @@ Definition syntax_ok_def: (* syntax expected by loop_remove *)
   (syntax_ok prog <=> F)
 End
 
+
+Definition survives_def:
+  (survives n (If c r ri p q cs) <=>
+     survives n p ∧ survives n q ∧ n ∈ domain cs) ∧
+  (survives n (Loop il p ol) <=>
+    n ∈ domain il ∧ n ∈ domain ol ∧ survives n p) ∧
+  (survives n (Call (SOME (m,cs)) trgt args NONE) <=>
+     n ∈ domain cs) ∧
+  (survives n (Call (SOME (m,cs)) trgt args (SOME (r,p,q,ps))) <=>
+     n ∈ domain cs ∧ n ∈ domain ps ∧ survives n p ∧ survives n q) ∧
+  (survives n (FFI fi ptr1 len1 ptr2 len2 cs) <=> n ∈ domain cs) ∧
+  (survives n (Mark p) <=> survives n p) ∧
+  (survives n (Seq p q) <=> survives n p ∧ survives n q) ∧
+  (survives n p <=> T)
+End
+
+
+Definition cut_sets_def:
+  (cut_sets l Skip = l) ∧
+  (cut_sets l (LocValue n m) = insert n () l) ∧
+  (cut_sets l (Assign n e) = insert n () l) ∧
+  (cut_sets l (LoadByte n m) = insert m () l) ∧
+  (cut_sets l (Seq p q) = cut_sets (cut_sets l p) q) ∧
+  (cut_sets l (If _ _ _ p q nl) = nl)
+End
+
+Definition comp_syntax_ok_def:
+  comp_syntax_ok l p <=>
+    p = Skip ∨
+    ?n m. p = LocValue n m ∨
+    ?n e. p = Assign n e ∨
+    ?n m. p = LoadByte n m ∨
+    ?c n m v v'. p = If c n (Reg m) (Assign n v) (Assign n v') (list_insert [n; m] l) ∨
+    ?q r. p = Seq q r ∧ comp_syntax_ok l q ∧ comp_syntax_ok (cut_sets l q) r
+Termination
+ cheat
+End
+
+
 Theorem evaluate_Loop_body_same:
   (∀(s:('a,'b)state). evaluate (body,s) = evaluate (body',s)) ⇒
   ∀(s:('a,'b)state). evaluate (Loop l1 body l2,s) = evaluate (Loop l1 body' l2,s)
@@ -228,6 +267,16 @@ Proof
   fs [get_vars_def]
 QED
 
+Theorem get_vars_clock_upd_eq:
+  !ns st l ck.
+   get_vars ns (st with clock := ck) =
+   get_vars ns st
+Proof
+  Induct >> rw [] >>
+  fs [get_vars_def]
+QED
+
+
 Theorem get_vars_local_update_some_eq:
   !ns vs st.
    ALL_DISTINCT ns /\ LENGTH ns = LENGTH vs ==>
@@ -246,21 +295,6 @@ Proof
   ho_match_mp_tac alist_insert_pull_insert >>
   fs []
 QED
-
-Definition survives_def:
-  (survives n (If c r ri p q cs) <=>
-     survives n p ∧ survives n q ∧ n ∈ domain cs) ∧
-  (survives n (Loop il p ol) <=>
-    n ∈ domain il ∧ n ∈ domain ol ∧ survives n p) ∧
-  (survives n (Call (SOME (m,cs)) trgt args NONE) <=>
-     n ∈ domain cs) ∧
-  (survives n (Call (SOME (m,cs)) trgt args (SOME (r,p,q,ps))) <=>
-     n ∈ domain cs ∧ n ∈ domain ps ∧ survives n p ∧ survives n q) ∧
-  (survives n (FFI fi ptr1 len1 ptr2 len2 cs) <=> n ∈ domain cs) ∧
-  (survives n (Mark p) <=> survives n p) ∧
-  (survives n (Seq p q) <=> survives n p ∧ survives n q) ∧
-  (survives n p <=> T)
-End
 
 
 Theorem unassigned_vars_evaluate_same:
@@ -336,85 +370,484 @@ Proof
   rveq >> fs [state_component_equality]
 QED
 
-(*
-Theorem unassigned_vars_evaluate_same:
-  !p s res t (l:sptree$num_set) n.
-   evaluate (p,s) = (res,t) /\
-   (res = NONE ∨ res = SOME Continue ∨ res = SOME Break) /\
-    ~MEM n (assigned_vars p) /\ (?v. lookup n (cutset l p) = SOME v) ==>
+
+Theorem evaluate_nested_seq_cases:
+  (!p q s st t.
+    evaluate (nested_seq (p ++ q), s) = (NONE, t) /\
+    evaluate (nested_seq p,s) = (NONE,st) ==>
+    evaluate (nested_seq q,st) = (NONE,t)) /\
+  (!p s st q.
+    evaluate (nested_seq p, s) = (NONE, st) ==>
+    evaluate (nested_seq (p ++ q), s) =  evaluate (nested_seq q, st)) /\
+  (!p s res st q.
+    evaluate (nested_seq p, s) = (res, st) /\
+    res <> NONE ==>
+    evaluate (nested_seq (p ++ q), s) =  evaluate (nested_seq p, s))
+Proof
+  rpt conj_tac >>
+  Induct >> rw []
+  >- fs [nested_seq_def, evaluate_def] >>
+  fs [nested_seq_def, evaluate_def] >>
+  pairarg_tac >> fs [] >>
+  FULL_CASE_TAC >> fs [] >>
+  res_tac >> fs []
+QED
+
+Theorem comp_syn_ok_basic_cases:
+  (!l. comp_syntax_ok l Skip) /\
+  (!l n m. comp_syntax_ok l (LocValue n m)) /\
+  (!l n e. comp_syntax_ok l (Assign n e)) /\
+  (!l n m. comp_syntax_ok l (LoadByte n m)) /\
+  (!l c n m v v'. comp_syntax_ok l (If c n (Reg m)
+       (Assign n v) (Assign n v') (list_insert [n; m] l)))
+Proof
+  rw [] >>
+  ntac 3 (fs [Once comp_syntax_ok_def])
+QED
+
+
+Theorem comp_syn_ok_seq:
+  !l p q. comp_syntax_ok l (Seq p q) ==>
+   comp_syntax_ok l p /\ comp_syntax_ok (cut_sets l p) q
+Proof
+  rw [] >>
+  fs [Once comp_syntax_ok_def]
+QED
+
+
+Theorem comp_syn_ok_if:
+  comp_syntax_ok l (If cmp n ri p q ns) ==>
+    ?v v' m. ri = Reg m /\ p = Assign n v /\
+       q = Assign n v' /\ ns = list_insert [n; m] l
+Proof
+  rw [] >>
+  fs [Once comp_syntax_ok_def]
+QED
+
+
+Theorem comp_syn_ok_seq2:
+  !l p q. comp_syntax_ok l p /\ comp_syntax_ok (cut_sets l p) q ==>
+   comp_syntax_ok l (Seq p q)
+Proof
+  rw [] >>
+  once_rewrite_tac [comp_syntax_ok_def] >>
+  fs []
+QED
+
+
+Theorem comp_syn_ok_nested_seq:
+  !p q l. comp_syntax_ok l (nested_seq p) ∧
+   comp_syntax_ok (cut_sets l (nested_seq p)) (nested_seq q) ==>
+   comp_syntax_ok l (nested_seq (p ++ q))
+Proof
+  Induct >> rw [] >>
+  fs [nested_seq_def] >>
+  fs [cut_sets_def] >>
+  drule comp_syn_ok_seq >>
+  strip_tac >> res_tac >> fs [] >>
+  metis_tac [comp_syn_ok_seq2]
+QED
+
+Theorem comp_syn_ok_nested_seq2:
+  !p q l. comp_syntax_ok l (nested_seq (p ++ q)) ==>
+   comp_syntax_ok l (nested_seq p) ∧
+   comp_syntax_ok (cut_sets l (nested_seq p)) (nested_seq q)
+Proof
+  Induct >> rw [] >>
+  fs [nested_seq_def, comp_syn_ok_basic_cases, cut_sets_def] >>
+  drule comp_syn_ok_seq >> strip_tac >> fs [] >>
+  metis_tac [comp_syn_ok_seq2]
+QED
+
+
+Theorem comp_syn_ok_cut_sets_nested_seq:
+  !p q l. comp_syntax_ok l (nested_seq p) ∧
+   comp_syntax_ok (cut_sets l (nested_seq p)) (nested_seq q) ==>
+   cut_sets l (nested_seq (p ++ q)) =
+   cut_sets (cut_sets l (nested_seq p)) (nested_seq q)
+Proof
+  Induct >> rw [] >>
+  fs [nested_seq_def]
+  >- fs [cut_sets_def] >>
+  fs [cut_sets_def] >>
+  drule comp_syn_ok_seq >>
+  strip_tac >>
+  res_tac >> fs []
+QED
+
+
+Theorem comp_syn_ok_cut_sets_nested_seq2:
+  !p q l. comp_syntax_ok l (nested_seq (p ++ q)) ==>
+   cut_sets l (nested_seq (p ++ q)) =
+   cut_sets (cut_sets l (nested_seq p)) (nested_seq q)
+Proof
+ metis_tac [comp_syn_ok_nested_seq2, comp_syn_ok_cut_sets_nested_seq]
+QED
+
+Theorem cut_sets_union_accumulate:
+  !p l. comp_syntax_ok l p ==>
+   ?(l' :sptree$num_set). cut_sets l p = union l l'
+Proof
+  Induct >> rw [] >>
+  TRY (fs [Once comp_syntax_ok_def] >> NO_TAC) >>
+  fs [cut_sets_def] >>
+  TRY (qexists_tac ‘LN’ >> fs [] >> NO_TAC) >>
+  TRY (
+  rename [‘insert vn () l’] >>
+  qexists_tac ‘insert vn () LN’ >>
+  fs [Once insert_union, union_num_set_sym] >> NO_TAC)
+  >- (
+   drule comp_syn_ok_seq >>
+   strip_tac >>
+   last_x_assum drule >>
+   strip_tac >> fs [] >>
+   last_x_assum (qspec_then ‘union l l'’ mp_tac) >>
+   fs [] >> strip_tac >>
+   qexists_tac ‘union l' l''’ >>
+   fs [] >> metis_tac [union_assoc]) >>
+  drule comp_syn_ok_if >>
+  strip_tac >> rveq >>
+  qexists_tac ‘insert m () (insert n () LN)’ >>
+  fs [list_insert_def] >>
+  metis_tac [union_insert_LN, insert_union, union_num_set_sym, union_assoc]
+QED
+
+
+Theorem cut_sets_union_domain_subset:
+  !p l. comp_syntax_ok l p ==>
+    domain l ⊆ domain (cut_sets l p)
+Proof
+  rw [] >>
+  drule cut_sets_union_accumulate >>
+  strip_tac >> fs [] >>
+  fs [domain_union]
+QED
+
+Theorem cut_sets_union_domain_union:
+  !p l. comp_syntax_ok l p ==>
+   ?(l' :sptree$num_set). domain (cut_sets l p) = domain l ∪ domain l'
+Proof
+  rw [] >>
+  drule cut_sets_union_accumulate >>
+  strip_tac >> fs [] >>
+  qexists_tac ‘l'’ >>
+  fs [domain_union]
+QED
+
+Theorem comp_syn_impl_cut_sets_subspt:
+  !p l. comp_syntax_ok l p ==>
+  subspt l (cut_sets l p)
+Proof
+  rw [] >>
+  drule cut_sets_union_accumulate >>
+  strip_tac >>
+  fs [subspt_union]
+QED
+
+Theorem comp_syn_cut_sets_mem_domain:
+  !p l n .
+   comp_syntax_ok l p /\ n ∈ domain l ==>
+    n ∈ domain (cut_sets l p)
+Proof
+  rw [] >>
+  drule cut_sets_union_domain_union >>
+  strip_tac >> fs []
+QED
+
+
+Theorem comp_syn_ok_upd_local_clock:
+  !p s res t l.
+    evaluate (p,s) = (res,t) /\
+    comp_syntax_ok l p ==>
+     t = s with <|locals := t.locals; clock := t.clock|>
+Proof
+  recInduct evaluate_ind >> rw [] >>
+  TRY (fs [Once comp_syntax_ok_def, every_prog_def] >> NO_TAC) >>
+  TRY (
+  fs [evaluate_def] >> rveq >>
+  TRY every_case_tac >> fs [set_var_def, state_component_equality] >> NO_TAC)
+  >- (
+   drule comp_syn_ok_seq >>
+   strip_tac >>
+   fs [evaluate_def] >>
+   pairarg_tac >> fs [] >>
+   FULL_CASE_TAC >> fs []  >> rveq >>
+   res_tac >> fs [state_component_equality]) >>
+  drule comp_syn_ok_if >>
+  strip_tac >> rveq >>
+  fs [evaluate_def] >>
+  every_case_tac >> fs [] >> rveq >>
+  fs [state_component_equality, evaluate_def, comp_syn_ok_basic_cases] >>
+  every_case_tac >>
+  fs [cut_res_def, cut_state_def, dec_clock_def, set_var_def] >>
+  every_case_tac >> fs [] >> rveq >> fs []
+QED
+
+
+Theorem assigned_vars_nested_seq_split:
+  !p q l.
+   comp_syntax_ok l (nested_seq p) /\
+   comp_syntax_ok (cut_sets l (nested_seq p)) (nested_seq q) ==>
+    assigned_vars (nested_seq (p ++ q)) =
+    assigned_vars (nested_seq p) ++ assigned_vars (nested_seq q)
+Proof
+  Induct >> rw [] >>
+  fs [nested_seq_def, assigned_vars_def] >>
+  drule comp_syn_ok_seq >> fs [] >>
+  strip_tac >>
+  fs [cut_sets_def] >> res_tac >> fs []
+QED
+
+Theorem assigned_vars_seq_split:
+  !q p l .
+   comp_syntax_ok l p /\ comp_syntax_ok (cut_sets l p) q ==>
+    assigned_vars (Seq p q) = assigned_vars p ++ assigned_vars q
+Proof
+  rw [] >> fs [assigned_vars_def, cut_sets_def]
+QED
+
+
+Theorem comp_syn_ok_lookup_locals_eq:
+  !p s res t l n.
+   evaluate (p,s) = (res,t) /\ res <> SOME TimeOut /\
+   comp_syntax_ok l p /\ n ∈ domain l /\
+    ~MEM n (assigned_vars p) ==>
   lookup n t.locals = lookup n s.locals
 Proof
-  recInduct evaluate_ind >>
-  rpt conj_tac >> rpt gen_tac >>
+  recInduct evaluate_ind >> rw [] >>
+  TRY (fs [Once comp_syntax_ok_def, every_prog_def] >> NO_TAC) >>
   TRY (
-  rw [] >>
-  fs [Once evaluate_def,AllCaseEqs(), set_var_def, set_globals_def,
-      dec_clock_def, assigned_vars_def, cutset_def] >>
-  rveq >> fs [lookup_insert, mem_store_def, AllCaseEqs()] >>
-  rveq >> fs [state_component_equality] >> NO_TAC) >>
-  TRY (
-  rename [‘Mark’] >>
-  rw [] >>
-  fs [Once evaluate_def,AllCaseEqs(), assigned_vars_def,
-      cutset_def, lookup_inter] >>
-  res_tac >> fs []) >>
-  TRY (
-  rename [‘FFI’] >>
-  rw [] >>
-  fs [Once evaluate_def,AllCaseEqs(), assigned_vars_def, cutset_def] >>
-  rveq >> fs [cut_state_def] >> rveq >> fs [lookup_inter,AllCaseEqs()] >>
-  cases_on ‘lookup n s.locals’ >> fs []) >>
+  fs [evaluate_def] >>
+  every_case_tac >> fs [] >> rveq >>
+  fs [set_var_def, assigned_vars_def, lookup_insert] >> NO_TAC)
+  >- (
+   drule comp_syn_ok_seq >>
+   strip_tac >>
+   fs [evaluate_def, assigned_vars_def] >>
+   pairarg_tac >> fs [AllCaseEqs ()] >> rveq >> fs []
+   >- (
+    qpat_x_assum ‘evaluate (_,s1) = _’ assume_tac  >>
+    drule evaluate_clock >> fs [] >>
+    strip_tac >> fs [] >>
+    dxrule comp_syn_ok_seq >>
+    strip_tac >>
+    first_x_assum drule >>
+    disch_then (qspec_then ‘n’ mp_tac) >>
+    fs [] >>
+    strip_tac >>
+    first_x_assum drule >>
+    disch_then (qspec_then ‘n’ mp_tac) >>
+    fs [] >>
+    impl_tac
+    >- (
+     qpat_x_assum ‘comp_syntax_ok l c1’ assume_tac >>
+     drule cut_sets_union_domain_union >>
+     strip_tac >> fs []) >>
+    fs []) >>
+   drule comp_syn_ok_seq >>
+   strip_tac >>
+   res_tac >> fs []) >>
+  drule evaluate_clock >> fs [] >>
+  strip_tac >> fs [] >>
+  drule comp_syn_ok_if >>
+  strip_tac >> rveq >> fs [] >>
+  fs [evaluate_def, assigned_vars_def] >>
+  fs [AllCaseEqs()]  >> rveq >> fs [domain_inter] >>
+  cases_on ‘word_cmp cmp x y’ >> fs [] >>
+  fs [evaluate_def, list_insert_def, AllCaseEqs()] >>
+  FULL_CASE_TAC >> fs [cut_res_def, set_var_def, dec_clock_def, cut_state_def] >>
+  FULL_CASE_TAC >> fs [] >> rveq >>
+  every_case_tac >> rfs [] >> rveq >> fs [] >>
+  fs [state_component_equality, lookup_inter, lookup_insert] >>
+  every_case_tac >> rfs [domain_lookup]
+QED
+
+Theorem eval_upd_clock_eq:
+  !t e ck. eval (t with clock := ck) e =  eval t e
+Proof
+  ho_match_mp_tac eval_ind >> rw [] >>
+  fs [eval_def]
+  >- (
+   every_case_tac >> fs [] >>
+   fs [mem_load_def]) >>
+  qsuff_tac ‘the_words (MAP (λa. eval (t with clock := ck) a) wexps) =
+             the_words (MAP (λa. eval t a) wexps)’ >>
+  fs [] >>
+  pop_assum mp_tac >>
+  qid_spec_tac ‘wexps’ >>
+  Induct >> rw [] >>
+  last_x_assum mp_tac >>
+  impl_tac >- metis_tac [] >>
+  strip_tac >> fs [wordSemTheory.the_words_def]
+QED
+
+(* should be trivial, but record updates are annoying *)
+
+Theorem eval_upd_locals_clock_eq:
+  !t e l ck. eval (t with <|locals := l; clock := ck|>) e =  eval (t with locals := l) e
+Proof
+  ho_match_mp_tac eval_ind >> rw [] >>
+  fs [eval_def]
+  >- (
+   every_case_tac >> fs [] >>
+   fs [mem_load_def]) >>
+  qsuff_tac ‘the_words (MAP (λa. eval (t with <|locals := l; clock := ck|>) a) wexps) =
+             the_words (MAP (λa. eval (t with locals := l) a) wexps)’ >>
+  fs [] >>
+  pop_assum mp_tac >>
+  qid_spec_tac ‘wexps’ >>
+  Induct >> rw [] >>
+  last_x_assum mp_tac >>
+  impl_tac >- metis_tac [] >>
+  strip_tac >> fs [wordSemTheory.the_words_def]
+QED
+
+Theorem cut_res_add_clock:
+  cut_res l (res,s) = (q,r) /\ q <> SOME TimeOut ==>
+  cut_res l (res,s with clock := ck + s.clock) =
+    (q,r with clock := ck + r.clock)
+Proof
+  rw [cut_res_def, cut_state_def] >>
+  ‘s.clock <> 0’ by fs [AllCaseEqs()] >>
+  fs [] >> rveq >> fs [dec_clock_def]
+QED
+
+Theorem evaluate_add_clock_eq:
+  !p t res st ck.
+   evaluate (p,t) = (res,st) /\ res <> SOME TimeOut ==>
+    evaluate (p,t with clock := t.clock + ck) = (res,st with clock := st.clock + ck)
+Proof
+  recInduct evaluate_ind >> rw [] >>
+  TRY (fs [Once evaluate_def] >> NO_TAC) >>
   TRY (
   rename [‘Seq’] >>
-  rw [] >>
-  fs [Once evaluate_def,AllCaseEqs(), assigned_vars_def,
-      cutset_def, lookup_inter] >>
-  pairarg_tac >> fs [AllCaseEqs()] >> rveq >>
-  res_tac >> fs [] >> res_tac >> fs [] >> NO_TAC) >>
+  fs [evaluate_def] >> pairarg_tac >> fs [] >>
+  pairarg_tac >> fs [] >> rveq >>
+  fs [AllCaseEqs ()] >> rveq >> fs [] >>
+  first_x_assum (qspec_then ‘ck’ mp_tac) >>
+  fs []) >>
   TRY (
   rename [‘If’] >>
-  rw [] >>
-  fs [Once evaluate_def, AllCaseEqs(), assigned_vars_def,
-      cutset_def] >> rveq >> fs [lookup_inter, AllCaseEqs()] >>
-  FULL_CASE_TAC >> fs [] >>
-  rename [‘cut_res _ (evaluate (c1,s))’] >>
-  cases_on ‘evaluate (c1,s)’ >> fs [] >>
-  cases_on ‘q’ >> fs [cut_res_def, AllCaseEqs(), dec_clock_def, cut_state_def] >>
-  rveq >> fs [lookup_inter, AllCaseEqs()] >>
-  res_tac >> rfs [] >> rw [] >>
-  cases_on ‘lookup n s.locals’ >> fs []) >>
+  fs [evaluate_def, AllCaseEqs ()] >>
+  rveq >> cases_on ‘ri’ >> fs [get_var_imm_def] >>
+  TOP_CASE_TAC >> cases_on ‘evaluate (c1,s)’ >> cases_on ‘evaluate (c2,s)’ >>
+  fs [cut_res_def, cut_state_def, AllCaseEqs (), dec_clock_def] >>
+  rveq >> fs []) >>
+  TRY (
+  rename [‘FFI’] >>
+  fs [evaluate_def, AllCaseEqs (), cut_state_def, call_env_def] >>
+  rveq >> fs []) >>
   TRY (
   rename [‘Loop’] >>
-  rw [] >>
-  qpat_x_assum ‘evaluate (Loop _ _ _,_) = _’ mp_tac >>
-  once_rewrite_tac [evaluate_def] >>
-  strip_tac >> fs [AllCaseEqs ()] >> rveq >>
-  fs [assigned_vars_def, cutset_def, cut_res_def, cut_state_def,
-      AllCaseEqs (), dec_clock_def] >>
-  rveq >> fs [] >>
-  fs [lookup_inter_alt] >>
-  res_tac >> rfs [domain_lookup] >>
-  res_tac >> fs []) >>
+  fs [Once evaluate_def] >>
+  TOP_CASE_TAC >> fs [] >>
+  cases_on ‘cut_res live_in ((NONE:'a result option),s)’ >>
+  fs [] >>
+  ‘q' <> SOME TimeOut’ by (
+    CCONTR_TAC >>
+    fs [cut_res_def, cut_state_def, AllCaseEqs(), dec_clock_def]) >>
+  drule cut_res_add_clock >>
+  disch_then (qspec_then ‘ck’ mp_tac) >> fs [] >>
+  strip_tac >> fs [] >> rveq >>
+  TOP_CASE_TAC >> fs [] >>
+  cases_on ‘evaluate (body,r')’ >> fs [] >> rveq >>
+  cases_on ‘q’ >> fs [] >>
+  cases_on ‘x’ >> fs [] >> rveq >> fs []
+  >- (imp_res_tac cut_res_add_clock >> res_tac >> fs []) >>
+  first_x_assum match_mp_tac >>
+  TOP_CASE_TAC >> fs [] >>
+  reverse TOP_CASE_TAC >> fs []
+  >- fs [Once evaluate_def] >>
+  TOP_CASE_TAC >> fs [] >>
+  TOP_CASE_TAC >> fs [] >>
+  fs [Once evaluate_def]) >>
+  TRY (
   rename [‘Call’] >>
-  rw [] >>
-  fs [evaluate_def] >>
-  FULL_CASE_TAC >> fs []
+  fs [evaluate_def, get_vars_clock_upd_eq, dec_clock_def] >>
+  ntac 4 (TOP_CASE_TAC >> fs [])
   >- (
-   every_case_tac >>
-   fs [cut_res_def, cut_state_def, AllCaseEqs()]) >>
-  fs [AllCaseEqs()] >> fs [] >> rveq >> fs [] >>
-  fs [cut_res_def, cut_state_def, AllCaseEqs(),
-      dec_clock_def, set_var_def] >> rveq >> fs [] >>
-  fs [cutset_def, lookup_inter, CaseEq "option"] >> rveq >>
-  fs [assigned_vars_def, lookup_insert,
-      lookup_inter_alt, domain_lookup] >>
-  rename [‘evaluate
-           (r,st with locals := insert n' retv (inter s.locals live))’] >>
-  cases_on ‘evaluate
-            (r,st with locals := insert n' retv (inter s.locals live))’ >>
-  fs [cut_res_def, cut_state_def, AllCaseEqs()] >> rveq >> fs [dec_clock_def] >>
-  res_tac >> fs [lookup_inter] >> TOP_CASE_TAC >> fs []
+   fs [AllCaseEqs()] >>
+   ‘s.clock <> 0’ by (
+     fs [AllCaseEqs()] >> rveq >> fs []) >>
+   rveq >> fs []) >>
+  TOP_CASE_TAC >> fs [] >>
+  cases_on ‘cut_res r' ((NONE:'a result option),s)’ >>
+  fs [] >>
+  ‘q'' <> SOME TimeOut’ by (
+    CCONTR_TAC >>
+    fs [cut_res_def, cut_state_def, AllCaseEqs(), dec_clock_def]) >>
+  drule cut_res_add_clock >>
+  disch_then (qspec_then ‘ck’ mp_tac) >> fs [] >>
+  strip_tac >> fs [] >>
+  TOP_CASE_TAC >> fs [] >>
+  cases_on ‘evaluate (r,r'' with locals := q)’ >> fs [] >> rveq >>
+  cases_on ‘q''’ >> fs [] >> rveq >>
+  cases_on ‘x'’ >> fs [] >> rveq >>
+  TOP_CASE_TAC >> fs [] >> rveq >>
+  fs [set_var_def] >>
+  rpt (TOP_CASE_TAC >> fs []) >>
+  qmatch_goalsub_abbrev_tac ‘cut_res nr (evaluate (rq,ar)) = _’ >>
+  qmatch_asmsub_abbrev_tac ‘evaluate (rq, lr)’ >>
+  cases_on ‘evaluate (rq, lr)’ >>
+  qmatch_asmsub_rename_tac ‘ evaluate _ = (tq,tr)’ >>
+  ‘tq <> SOME TimeOut’ by (
+    CCONTR_TAC >>
+    unabbrev_all_tac >>
+    fs [cut_res_def, cut_state_def, AllCaseEqs(), dec_clock_def]) >>
+  first_x_assum (qspecl_then [‘tq’, ‘tr’, ‘ck’] mp_tac) >>
+  fs [] >> strip_tac >>
+  imp_res_tac cut_res_add_clock >>
+  res_tac >> fs []) >>
+  fs [evaluate_def, eval_upd_clock_eq, AllCaseEqs () ,
+      set_var_def, mem_store_def, set_globals_def,
+      call_env_def, dec_clock_def] >> rveq >>
+  fs [state_component_equality]
 QED
-*)
+
+Theorem evaluate_nested_seq_comb_seq:
+  !p q t.
+   evaluate (Seq (nested_seq p) (nested_seq q), t) =
+   evaluate (nested_seq (p ++ q), t)
+Proof
+  Induct >> rw [] >>
+  fs [nested_seq_def, evaluate_def] >>
+  pairarg_tac >> fs [] >>
+  pairarg_tac >> fs [] >>
+  cases_on ‘res' = NONE’ >> fs [] >> rveq >> fs [] >>
+  first_x_assum (qspecl_then [‘q’,‘s1'’] mp_tac) >>
+  fs []
+QED
+
+
+Theorem nested_seq_pure_evaluation:
+  !p q t r st l m e v ck ck'.
+  evaluate (nested_seq p,t with clock := ck + t.clock) = (NONE,st) /\
+  evaluate (nested_seq q,st with clock := ck' + st.clock) = (NONE,r) /\
+  comp_syntax_ok l (nested_seq p) /\
+  comp_syntax_ok (cut_sets l (nested_seq p)) (nested_seq q) /\
+  (!n. MEM n (assigned_vars (nested_seq p)) ==> n < m) /\
+  (!n. MEM n (assigned_vars (nested_seq q)) ==> m <= n) /\
+  (!n. MEM n (locals_touched e) ==> n < m /\ n ∈ domain (cut_sets l (nested_seq p))) /\
+   eval st e = SOME v ==>
+    eval r e = SOME v
+Proof
+  rw [] >>
+  drule_all comp_syn_ok_upd_local_clock >>
+  fs [] >> strip_tac >>
+  ‘st.globals = r.globals /\ st.memory = r.memory /\
+   st.mdomain = r.mdomain’ by fs [state_component_equality] >>
+  drule locals_touched_eq_eval_eq >> fs [] >>
+  disch_then (qspec_then ‘e’ mp_tac) >> fs [] >>
+  impl_tac
+  >- (
+   rw []  >>
+   drule comp_syn_ok_lookup_locals_eq >>
+   disch_then (qspecl_then [‘cut_sets l (nested_seq p)’, ‘n’] mp_tac) >>
+   impl_tac
+   >- (
+    fs [] >>
+    CCONTR_TAC >> fs [] >>
+    res_tac >> fs []) >> fs []) >> fs []
+QED
 
 val _ = export_theory();
